src/coq/Handlers/Concretization.v
@@ -79,14 +79,14 @@ Module Type ConcretizationBase (LP : LLVMParams) (MP : MemoryParams LP) (Byte : 
     | DVALUE_I16 i1, DVALUE_I16 i2
     | DVALUE_I32 i1, DVALUE_I32 i2
     | DVALUE_I64 i1, DVALUE_I64 i2
-    | DVALUE_IPTR i1, DVALUE_IPTR i2 => ret (eval_int_icmp icmp i1 i2)
+    | DVALUE_IPTR i1, DVALUE_IPTR i2 => eval_int_icmp icmp i1 i2
     | DVALUE_Poison t1, DVALUE_Poison t2 => ret (DVALUE_Poison t1)
     | DVALUE_Poison t, _ => if is_DVALUE_IX v2 then ret (DVALUE_Poison t) else raise_error "ill_typed-iop"
     | _, DVALUE_Poison t => if is_DVALUE_IX v1 then ret (DVALUE_Poison t) else raise_error "ill_typed-iop"
     | DVALUE_Addr a1, DVALUE_Addr a2 =>
         let i1 := ptr_to_int a1 in
         let i2 := ptr_to_int a2 in
-        ret (eval_int_icmp icmp i1 i2)
+        eval_int_icmp icmp i1 i2
     | _, _ => raise_error ("ill_typed-icmp: " ++ show_dvalue v1 ++ ", " ++ show_dvalue v2)
     end.
   Arguments eval_icmp _ _ _ : simpl nomatch.
@@ -690,14 +690,14 @@ Module MakeBase (LP : LLVMParams) (MP : MemoryParams LP) (Byte : ByteModule LP.A
     | DVALUE_I16 i1, DVALUE_I16 i2
     | DVALUE_I32 i1, DVALUE_I32 i2
     | DVALUE_I64 i1, DVALUE_I64 i2
-    | DVALUE_IPTR i1, DVALUE_IPTR i2 => ret (eval_int_icmp icmp i1 i2)
+    | DVALUE_IPTR i1, DVALUE_IPTR i2 => eval_int_icmp icmp i1 i2
     | DVALUE_Poison t1, DVALUE_Poison t2 => ret (DVALUE_Poison t1)
     | DVALUE_Poison t, _ => if is_DVALUE_IX v2 then ret (DVALUE_Poison t) else raise_error "ill_typed-iop"
     | _, DVALUE_Poison t => if is_DVALUE_IX v1 then ret (DVALUE_Poison t) else raise_error "ill_typed-iop"
     | DVALUE_Addr a1, DVALUE_Addr a2 =>
         let i1 := ptr_to_int a1 in
         let i2 := ptr_to_int a2 in
-        ret (eval_int_icmp icmp i1 i2)
+        eval_int_icmp icmp i1 i2
     | _, _ => raise_error ("ill_typed-icmp: " ++ show_dvalue v1 ++ ", " ++ show_dvalue v2)
     end.
   Arguments eval_icmp _ _ _ : simpl nomatch.
